Added full schoolbook iteration
Signed-off-by: dkostic <dkostic@amazon.com>

x86/proofs/mlkem_basemul_k2.ml
@@ -12,8 +12,8 @@ needs "common/mlkem_mldsa.ml";;
 
 print_literal_from_elf "x86/mlkem/mlkem_basemul_k2.o";;
 
-let mlkem_basemul_k2_mc =
-  define_assert_from_elf "mlkem_basemul_k2_mc" "x86/mlkem/mlkem_basemul_k2.o"
+let mlkem_basemul_k2_mc2 =
+  define_assert_from_elf "mlkem_basemul_k2_mc2" "x86/mlkem/mlkem_basemul_k2.o"
 [
   0xf3; 0x0f; 0x1e; 0xfa;  (* ENDBR64 *)
   0xb8; 0x01; 0x0d; 0x01; 0x0d;
@@ -112,11 +112,281 @@ let mlkem_basemul_k2_mc =
                            (* VMOVDQA (Memop Word256 (%% (rdi,64))) (%_% ymm7) *)
   0xc5; 0x7d; 0x7f; 0x4f; 0x60;
                            (* VMOVDQA (Memop Word256 (%% (rdi,96))) (%_% ymm9) *)
+  0xc5; 0xfd; 0x6f; 0x96; 0x80; 0x00; 0x00; 0x00;
+                           (* VMOVDQA (%_% ymm2) (Memop Word256 (%% (rsi,128))) *)
+  0xc5; 0xfd; 0x6f; 0x9e; 0xa0; 0x00; 0x00; 0x00;
+                           (* VMOVDQA (%_% ymm3) (Memop Word256 (%% (rsi,160))) *)
+  0xc5; 0xfd; 0x6f; 0xa2; 0x80; 0x00; 0x00; 0x00;
+                           (* VMOVDQA (%_% ymm4) (Memop Word256 (%% (rdx,128))) *)
+  0xc5; 0xfd; 0x6f; 0xaa; 0xa0; 0x00; 0x00; 0x00;
+                           (* VMOVDQA (%_% ymm5) (Memop Word256 (%% (rdx,160))) *)
+  0xc5; 0xfd; 0x6f; 0x71; 0x40;
+                           (* VMOVDQA (%_% ymm6) (Memop Word256 (%% (rcx,64))) *)
+  0xc5; 0x75; 0xd5; 0xea;  (* VPMULLW (%_% ymm13) (%_% ymm1) (%_% ymm2) *)
+  0xc5; 0x75; 0xd5; 0xf3;  (* VPMULLW (%_% ymm14) (%_% ymm1) (%_% ymm3) *)
+  0xc4; 0xc1; 0x5d; 0xd5; 0xfd;
+                           (* VPMULLW (%_% ymm7) (%_% ymm4) (%_% ymm13) *)
+  0xc4; 0x41; 0x55; 0xd5; 0xcd;
+                           (* VPMULLW (%_% ymm9) (%_% ymm5) (%_% ymm13) *)
+  0xc4; 0x41; 0x4d; 0xd5; 0xc6;
+                           (* VPMULLW (%_% ymm8) (%_% ymm6) (%_% ymm14) *)
+  0xc4; 0x41; 0x5d; 0xd5; 0xd6;
+                           (* VPMULLW (%_% ymm10) (%_% ymm4) (%_% ymm14) *)
+  0xc5; 0xfd; 0xe5; 0xff;  (* VPMULHW (%_% ymm7) (%_% ymm0) (%_% ymm7) *)
+  0xc4; 0x41; 0x7d; 0xe5; 0xc9;
+                           (* VPMULHW (%_% ymm9) (%_% ymm0) (%_% ymm9) *)
+  0xc4; 0x41; 0x7d; 0xe5; 0xc0;
+                           (* VPMULHW (%_% ymm8) (%_% ymm0) (%_% ymm8) *)
+  0xc4; 0x41; 0x7d; 0xe5; 0xd2;
+                           (* VPMULHW (%_% ymm10) (%_% ymm0) (%_% ymm10) *)
+  0xc5; 0x5d; 0xe5; 0xda;  (* VPMULHW (%_% ymm11) (%_% ymm4) (%_% ymm2) *)
+  0xc5; 0x55; 0xe5; 0xe2;  (* VPMULHW (%_% ymm12) (%_% ymm5) (%_% ymm2) *)
+  0xc5; 0x4d; 0xe5; 0xeb;  (* VPMULHW (%_% ymm13) (%_% ymm6) (%_% ymm3) *)
+  0xc5; 0x5d; 0xe5; 0xf3;  (* VPMULHW (%_% ymm14) (%_% ymm4) (%_% ymm3) *)
+  0xc5; 0xa5; 0xf9; 0xff;  (* VPSUBW (%_% ymm7) (%_% ymm11) (%_% ymm7) *)
+  0xc4; 0x41; 0x1d; 0xf9; 0xc9;
+                           (* VPSUBW (%_% ymm9) (%_% ymm12) (%_% ymm9) *)
+  0xc4; 0x41; 0x15; 0xf9; 0xc0;
+                           (* VPSUBW (%_% ymm8) (%_% ymm13) (%_% ymm8) *)
+  0xc4; 0x41; 0x0d; 0xf9; 0xd2;
+                           (* VPSUBW (%_% ymm10) (%_% ymm14) (%_% ymm10) *)
+  0xc5; 0xbd; 0xfd; 0xff;  (* VPADDW (%_% ymm7) (%_% ymm8) (%_% ymm7) *)
+  0xc4; 0x41; 0x2d; 0xfd; 0xc9;
+                           (* VPADDW (%_% ymm9) (%_% ymm10) (%_% ymm9) *)
+  0xc5; 0xfd; 0x7f; 0xbf; 0x80; 0x00; 0x00; 0x00;
+                           (* VMOVDQA (Memop Word256 (%% (rdi,128))) (%_% ymm7) *)
+  0xc5; 0x7d; 0x7f; 0x8f; 0xa0; 0x00; 0x00; 0x00;
+                           (* VMOVDQA (Memop Word256 (%% (rdi,160))) (%_% ymm9) *)
+  0xc5; 0xfd; 0x6f; 0x96; 0xc0; 0x00; 0x00; 0x00;
+                           (* VMOVDQA (%_% ymm2) (Memop Word256 (%% (rsi,192))) *)
+  0xc5; 0xfd; 0x6f; 0x9e; 0xe0; 0x00; 0x00; 0x00;
+                           (* VMOVDQA (%_% ymm3) (Memop Word256 (%% (rsi,224))) *)
+  0xc5; 0xfd; 0x6f; 0xa2; 0xc0; 0x00; 0x00; 0x00;
+                           (* VMOVDQA (%_% ymm4) (Memop Word256 (%% (rdx,192))) *)
+  0xc5; 0xfd; 0x6f; 0xaa; 0xe0; 0x00; 0x00; 0x00;
+                           (* VMOVDQA (%_% ymm5) (Memop Word256 (%% (rdx,224))) *)
+  0xc5; 0xfd; 0x6f; 0x71; 0x60;
+                           (* VMOVDQA (%_% ymm6) (Memop Word256 (%% (rcx,96))) *)
+  0xc5; 0x75; 0xd5; 0xea;  (* VPMULLW (%_% ymm13) (%_% ymm1) (%_% ymm2) *)
+  0xc5; 0x75; 0xd5; 0xf3;  (* VPMULLW (%_% ymm14) (%_% ymm1) (%_% ymm3) *)
+  0xc4; 0xc1; 0x5d; 0xd5; 0xfd;
+                           (* VPMULLW (%_% ymm7) (%_% ymm4) (%_% ymm13) *)
+  0xc4; 0x41; 0x55; 0xd5; 0xcd;
+                           (* VPMULLW (%_% ymm9) (%_% ymm5) (%_% ymm13) *)
+  0xc4; 0x41; 0x4d; 0xd5; 0xc6;
+                           (* VPMULLW (%_% ymm8) (%_% ymm6) (%_% ymm14) *)
+  0xc4; 0x41; 0x5d; 0xd5; 0xd6;
+                           (* VPMULLW (%_% ymm10) (%_% ymm4) (%_% ymm14) *)
+  0xc5; 0xfd; 0xe5; 0xff;  (* VPMULHW (%_% ymm7) (%_% ymm0) (%_% ymm7) *)
+  0xc4; 0x41; 0x7d; 0xe5; 0xc9;
+                           (* VPMULHW (%_% ymm9) (%_% ymm0) (%_% ymm9) *)
+  0xc4; 0x41; 0x7d; 0xe5; 0xc0;
+                           (* VPMULHW (%_% ymm8) (%_% ymm0) (%_% ymm8) *)
+  0xc4; 0x41; 0x7d; 0xe5; 0xd2;
+                           (* VPMULHW (%_% ymm10) (%_% ymm0) (%_% ymm10) *)
+  0xc5; 0x5d; 0xe5; 0xda;  (* VPMULHW (%_% ymm11) (%_% ymm4) (%_% ymm2) *)
+  0xc5; 0x55; 0xe5; 0xe2;  (* VPMULHW (%_% ymm12) (%_% ymm5) (%_% ymm2) *)
+  0xc5; 0x4d; 0xe5; 0xeb;  (* VPMULHW (%_% ymm13) (%_% ymm6) (%_% ymm3) *)
+  0xc5; 0x5d; 0xe5; 0xf3;  (* VPMULHW (%_% ymm14) (%_% ymm4) (%_% ymm3) *)
+  0xc5; 0xa5; 0xf9; 0xff;  (* VPSUBW (%_% ymm7) (%_% ymm11) (%_% ymm7) *)
+  0xc4; 0x41; 0x1d; 0xf9; 0xc9;
+                           (* VPSUBW (%_% ymm9) (%_% ymm12) (%_% ymm9) *)
+  0xc4; 0x41; 0x3d; 0xf9; 0xc5;
+                           (* VPSUBW (%_% ymm8) (%_% ymm8) (%_% ymm13) *)
+  0xc4; 0x41; 0x0d; 0xf9; 0xd2;
+                           (* VPSUBW (%_% ymm10) (%_% ymm14) (%_% ymm10) *)
+  0xc5; 0xbd; 0xfd; 0xff;  (* VPADDW (%_% ymm7) (%_% ymm8) (%_% ymm7) *)
+  0xc4; 0x41; 0x2d; 0xfd; 0xc9;
+                           (* VPADDW (%_% ymm9) (%_% ymm10) (%_% ymm9) *)
+  0xc5; 0xfd; 0x7f; 0xbf; 0xc0; 0x00; 0x00; 0x00;
+                           (* VMOVDQA (Memop Word256 (%% (rdi,192))) (%_% ymm7) *)
+  0xc5; 0x7d; 0x7f; 0x8f; 0xe0; 0x00; 0x00; 0x00;
+                           (* VMOVDQA (Memop Word256 (%% (rdi,224))) (%_% ymm9) *)
+  0xc5; 0xfd; 0x6f; 0x96; 0x00; 0x01; 0x00; 0x00;
+                           (* VMOVDQA (%_% ymm2) (Memop Word256 (%% (rsi,256))) *)
+  0xc5; 0xfd; 0x6f; 0x9e; 0x20; 0x01; 0x00; 0x00;
+                           (* VMOVDQA (%_% ymm3) (Memop Word256 (%% (rsi,288))) *)
+  0xc5; 0xfd; 0x6f; 0xa2; 0x00; 0x01; 0x00; 0x00;
+                           (* VMOVDQA (%_% ymm4) (Memop Word256 (%% (rdx,256))) *)
+  0xc5; 0xfd; 0x6f; 0xaa; 0x20; 0x01; 0x00; 0x00;
+                           (* VMOVDQA (%_% ymm5) (Memop Word256 (%% (rdx,288))) *)
+  0xc5; 0xfd; 0x6f; 0xb1; 0x80; 0x00; 0x00; 0x00;
+                           (* VMOVDQA (%_% ymm6) (Memop Word256 (%% (rcx,128))) *)
+  0xc5; 0x75; 0xd5; 0xea;  (* VPMULLW (%_% ymm13) (%_% ymm1) (%_% ymm2) *)
+  0xc5; 0x75; 0xd5; 0xf3;  (* VPMULLW (%_% ymm14) (%_% ymm1) (%_% ymm3) *)
+  0xc4; 0xc1; 0x5d; 0xd5; 0xfd;
+                           (* VPMULLW (%_% ymm7) (%_% ymm4) (%_% ymm13) *)
+  0xc4; 0x41; 0x55; 0xd5; 0xcd;
+                           (* VPMULLW (%_% ymm9) (%_% ymm5) (%_% ymm13) *)
+  0xc4; 0x41; 0x4d; 0xd5; 0xc6;
+                           (* VPMULLW (%_% ymm8) (%_% ymm6) (%_% ymm14) *)
+  0xc4; 0x41; 0x5d; 0xd5; 0xd6;
+                           (* VPMULLW (%_% ymm10) (%_% ymm4) (%_% ymm14) *)
+  0xc5; 0xfd; 0xe5; 0xff;  (* VPMULHW (%_% ymm7) (%_% ymm0) (%_% ymm7) *)
+  0xc4; 0x41; 0x7d; 0xe5; 0xc9;
+                           (* VPMULHW (%_% ymm9) (%_% ymm0) (%_% ymm9) *)
+  0xc4; 0x41; 0x7d; 0xe5; 0xc0;
+                           (* VPMULHW (%_% ymm8) (%_% ymm0) (%_% ymm8) *)
+  0xc4; 0x41; 0x7d; 0xe5; 0xd2;
+                           (* VPMULHW (%_% ymm10) (%_% ymm0) (%_% ymm10) *)
+  0xc5; 0x5d; 0xe5; 0xda;  (* VPMULHW (%_% ymm11) (%_% ymm4) (%_% ymm2) *)
+  0xc5; 0x55; 0xe5; 0xe2;  (* VPMULHW (%_% ymm12) (%_% ymm5) (%_% ymm2) *)
+  0xc5; 0x4d; 0xe5; 0xeb;  (* VPMULHW (%_% ymm13) (%_% ymm6) (%_% ymm3) *)
+  0xc5; 0x5d; 0xe5; 0xf3;  (* VPMULHW (%_% ymm14) (%_% ymm4) (%_% ymm3) *)
+  0xc5; 0xa5; 0xf9; 0xff;  (* VPSUBW (%_% ymm7) (%_% ymm11) (%_% ymm7) *)
+  0xc4; 0x41; 0x1d; 0xf9; 0xc9;
+                           (* VPSUBW (%_% ymm9) (%_% ymm12) (%_% ymm9) *)
+  0xc4; 0x41; 0x15; 0xf9; 0xc0;
+                           (* VPSUBW (%_% ymm8) (%_% ymm13) (%_% ymm8) *)
+  0xc4; 0x41; 0x0d; 0xf9; 0xd2;
+                           (* VPSUBW (%_% ymm10) (%_% ymm14) (%_% ymm10) *)
+  0xc5; 0xbd; 0xfd; 0xff;  (* VPADDW (%_% ymm7) (%_% ymm8) (%_% ymm7) *)
+  0xc4; 0x41; 0x2d; 0xfd; 0xc9;
+                           (* VPADDW (%_% ymm9) (%_% ymm10) (%_% ymm9) *)
+  0xc5; 0xfd; 0x7f; 0xbf; 0x00; 0x01; 0x00; 0x00;
+                           (* VMOVDQA (Memop Word256 (%% (rdi,256))) (%_% ymm7) *)
+  0xc5; 0x7d; 0x7f; 0x8f; 0x20; 0x01; 0x00; 0x00;
+                           (* VMOVDQA (Memop Word256 (%% (rdi,288))) (%_% ymm9) *)
+  0xc5; 0xfd; 0x6f; 0x96; 0x40; 0x01; 0x00; 0x00;
+                           (* VMOVDQA (%_% ymm2) (Memop Word256 (%% (rsi,320))) *)
+  0xc5; 0xfd; 0x6f; 0x9e; 0x60; 0x01; 0x00; 0x00;
+                           (* VMOVDQA (%_% ymm3) (Memop Word256 (%% (rsi,352))) *)
+  0xc5; 0xfd; 0x6f; 0xa2; 0x40; 0x01; 0x00; 0x00;
+                           (* VMOVDQA (%_% ymm4) (Memop Word256 (%% (rdx,320))) *)
+  0xc5; 0xfd; 0x6f; 0xaa; 0x60; 0x01; 0x00; 0x00;
+                           (* VMOVDQA (%_% ymm5) (Memop Word256 (%% (rdx,352))) *)
+  0xc5; 0xfd; 0x6f; 0xb1; 0xa0; 0x00; 0x00; 0x00;
+                           (* VMOVDQA (%_% ymm6) (Memop Word256 (%% (rcx,160))) *)
+  0xc5; 0x75; 0xd5; 0xea;  (* VPMULLW (%_% ymm13) (%_% ymm1) (%_% ymm2) *)
+  0xc5; 0x75; 0xd5; 0xf3;  (* VPMULLW (%_% ymm14) (%_% ymm1) (%_% ymm3) *)
+  0xc4; 0xc1; 0x5d; 0xd5; 0xfd;
+                           (* VPMULLW (%_% ymm7) (%_% ymm4) (%_% ymm13) *)
+  0xc4; 0x41; 0x55; 0xd5; 0xcd;
+                           (* VPMULLW (%_% ymm9) (%_% ymm5) (%_% ymm13) *)
+  0xc4; 0x41; 0x4d; 0xd5; 0xc6;
+                           (* VPMULLW (%_% ymm8) (%_% ymm6) (%_% ymm14) *)
+  0xc4; 0x41; 0x5d; 0xd5; 0xd6;
+                           (* VPMULLW (%_% ymm10) (%_% ymm4) (%_% ymm14) *)
+  0xc5; 0xfd; 0xe5; 0xff;  (* VPMULHW (%_% ymm7) (%_% ymm0) (%_% ymm7) *)
+  0xc4; 0x41; 0x7d; 0xe5; 0xc9;
+                           (* VPMULHW (%_% ymm9) (%_% ymm0) (%_% ymm9) *)
+  0xc4; 0x41; 0x7d; 0xe5; 0xc0;
+                           (* VPMULHW (%_% ymm8) (%_% ymm0) (%_% ymm8) *)
+  0xc4; 0x41; 0x7d; 0xe5; 0xd2;
+                           (* VPMULHW (%_% ymm10) (%_% ymm0) (%_% ymm10) *)
+  0xc5; 0x5d; 0xe5; 0xda;  (* VPMULHW (%_% ymm11) (%_% ymm4) (%_% ymm2) *)
+  0xc5; 0x55; 0xe5; 0xe2;  (* VPMULHW (%_% ymm12) (%_% ymm5) (%_% ymm2) *)
+  0xc5; 0x4d; 0xe5; 0xeb;  (* VPMULHW (%_% ymm13) (%_% ymm6) (%_% ymm3) *)
+  0xc5; 0x5d; 0xe5; 0xf3;  (* VPMULHW (%_% ymm14) (%_% ymm4) (%_% ymm3) *)
+  0xc5; 0xa5; 0xf9; 0xff;  (* VPSUBW (%_% ymm7) (%_% ymm11) (%_% ymm7) *)
+  0xc4; 0x41; 0x1d; 0xf9; 0xc9;
+                           (* VPSUBW (%_% ymm9) (%_% ymm12) (%_% ymm9) *)
+  0xc4; 0x41; 0x3d; 0xf9; 0xc5;
+                           (* VPSUBW (%_% ymm8) (%_% ymm8) (%_% ymm13) *)
+  0xc4; 0x41; 0x0d; 0xf9; 0xd2;
+                           (* VPSUBW (%_% ymm10) (%_% ymm14) (%_% ymm10) *)
+  0xc5; 0xbd; 0xfd; 0xff;  (* VPADDW (%_% ymm7) (%_% ymm8) (%_% ymm7) *)
+  0xc4; 0x41; 0x2d; 0xfd; 0xc9;
+                           (* VPADDW (%_% ymm9) (%_% ymm10) (%_% ymm9) *)
+  0xc5; 0xfd; 0x7f; 0xbf; 0x40; 0x01; 0x00; 0x00;
+                           (* VMOVDQA (Memop Word256 (%% (rdi,320))) (%_% ymm7) *)
+  0xc5; 0x7d; 0x7f; 0x8f; 0x60; 0x01; 0x00; 0x00;
+                           (* VMOVDQA (Memop Word256 (%% (rdi,352))) (%_% ymm9) *)
+  0xc5; 0xfd; 0x6f; 0x96; 0x80; 0x01; 0x00; 0x00;
+                           (* VMOVDQA (%_% ymm2) (Memop Word256 (%% (rsi,384))) *)
+  0xc5; 0xfd; 0x6f; 0x9e; 0xa0; 0x01; 0x00; 0x00;
+                           (* VMOVDQA (%_% ymm3) (Memop Word256 (%% (rsi,416))) *)
+  0xc5; 0xfd; 0x6f; 0xa2; 0x80; 0x01; 0x00; 0x00;
+                           (* VMOVDQA (%_% ymm4) (Memop Word256 (%% (rdx,384))) *)
+  0xc5; 0xfd; 0x6f; 0xaa; 0xa0; 0x01; 0x00; 0x00;
+                           (* VMOVDQA (%_% ymm5) (Memop Word256 (%% (rdx,416))) *)
+  0xc5; 0xfd; 0x6f; 0xb1; 0xc0; 0x00; 0x00; 0x00;
+                           (* VMOVDQA (%_% ymm6) (Memop Word256 (%% (rcx,192))) *)
+  0xc5; 0x75; 0xd5; 0xea;  (* VPMULLW (%_% ymm13) (%_% ymm1) (%_% ymm2) *)
+  0xc5; 0x75; 0xd5; 0xf3;  (* VPMULLW (%_% ymm14) (%_% ymm1) (%_% ymm3) *)
+  0xc4; 0xc1; 0x5d; 0xd5; 0xfd;
+                           (* VPMULLW (%_% ymm7) (%_% ymm4) (%_% ymm13) *)
+  0xc4; 0x41; 0x55; 0xd5; 0xcd;
+                           (* VPMULLW (%_% ymm9) (%_% ymm5) (%_% ymm13) *)
+  0xc4; 0x41; 0x4d; 0xd5; 0xc6;
+                           (* VPMULLW (%_% ymm8) (%_% ymm6) (%_% ymm14) *)
+  0xc4; 0x41; 0x5d; 0xd5; 0xd6;
+                           (* VPMULLW (%_% ymm10) (%_% ymm4) (%_% ymm14) *)
+  0xc5; 0xfd; 0xe5; 0xff;  (* VPMULHW (%_% ymm7) (%_% ymm0) (%_% ymm7) *)
+  0xc4; 0x41; 0x7d; 0xe5; 0xc9;
+                           (* VPMULHW (%_% ymm9) (%_% ymm0) (%_% ymm9) *)
+  0xc4; 0x41; 0x7d; 0xe5; 0xc0;
+                           (* VPMULHW (%_% ymm8) (%_% ymm0) (%_% ymm8) *)
+  0xc4; 0x41; 0x7d; 0xe5; 0xd2;
+                           (* VPMULHW (%_% ymm10) (%_% ymm0) (%_% ymm10) *)
+  0xc5; 0x5d; 0xe5; 0xda;  (* VPMULHW (%_% ymm11) (%_% ymm4) (%_% ymm2) *)
+  0xc5; 0x55; 0xe5; 0xe2;  (* VPMULHW (%_% ymm12) (%_% ymm5) (%_% ymm2) *)
+  0xc5; 0x4d; 0xe5; 0xeb;  (* VPMULHW (%_% ymm13) (%_% ymm6) (%_% ymm3) *)
+  0xc5; 0x5d; 0xe5; 0xf3;  (* VPMULHW (%_% ymm14) (%_% ymm4) (%_% ymm3) *)
+  0xc5; 0xa5; 0xf9; 0xff;  (* VPSUBW (%_% ymm7) (%_% ymm11) (%_% ymm7) *)
+  0xc4; 0x41; 0x1d; 0xf9; 0xc9;
+                           (* VPSUBW (%_% ymm9) (%_% ymm12) (%_% ymm9) *)
+  0xc4; 0x41; 0x15; 0xf9; 0xc0;
+                           (* VPSUBW (%_% ymm8) (%_% ymm13) (%_% ymm8) *)
+  0xc4; 0x41; 0x0d; 0xf9; 0xd2;
+                           (* VPSUBW (%_% ymm10) (%_% ymm14) (%_% ymm10) *)
+  0xc5; 0xbd; 0xfd; 0xff;  (* VPADDW (%_% ymm7) (%_% ymm8) (%_% ymm7) *)
+  0xc4; 0x41; 0x2d; 0xfd; 0xc9;
+                           (* VPADDW (%_% ymm9) (%_% ymm10) (%_% ymm9) *)
+  0xc5; 0xfd; 0x7f; 0xbf; 0x80; 0x01; 0x00; 0x00;
+                           (* VMOVDQA (Memop Word256 (%% (rdi,384))) (%_% ymm7) *)
+  0xc5; 0x7d; 0x7f; 0x8f; 0xa0; 0x01; 0x00; 0x00;
+                           (* VMOVDQA (Memop Word256 (%% (rdi,416))) (%_% ymm9) *)
+  0xc5; 0xfd; 0x6f; 0x96; 0xc0; 0x01; 0x00; 0x00;
+                           (* VMOVDQA (%_% ymm2) (Memop Word256 (%% (rsi,448))) *)
+  0xc5; 0xfd; 0x6f; 0x9e; 0xe0; 0x01; 0x00; 0x00;
+                           (* VMOVDQA (%_% ymm3) (Memop Word256 (%% (rsi,480))) *)
+  0xc5; 0xfd; 0x6f; 0xa2; 0xc0; 0x01; 0x00; 0x00;
+                           (* VMOVDQA (%_% ymm4) (Memop Word256 (%% (rdx,448))) *)
+  0xc5; 0xfd; 0x6f; 0xaa; 0xe0; 0x01; 0x00; 0x00;
+                           (* VMOVDQA (%_% ymm5) (Memop Word256 (%% (rdx,480))) *)
+  0xc5; 0xfd; 0x6f; 0xb1; 0xe0; 0x00; 0x00; 0x00;
+                           (* VMOVDQA (%_% ymm6) (Memop Word256 (%% (rcx,224))) *)
+  0xc5; 0x75; 0xd5; 0xea;  (* VPMULLW (%_% ymm13) (%_% ymm1) (%_% ymm2) *)
+  0xc5; 0x75; 0xd5; 0xf3;  (* VPMULLW (%_% ymm14) (%_% ymm1) (%_% ymm3) *)
+  0xc4; 0xc1; 0x5d; 0xd5; 0xfd;
+                           (* VPMULLW (%_% ymm7) (%_% ymm4) (%_% ymm13) *)
+  0xc4; 0x41; 0x55; 0xd5; 0xcd;
+                           (* VPMULLW (%_% ymm9) (%_% ymm5) (%_% ymm13) *)
+  0xc4; 0x41; 0x4d; 0xd5; 0xc6;
+                           (* VPMULLW (%_% ymm8) (%_% ymm6) (%_% ymm14) *)
+  0xc4; 0x41; 0x5d; 0xd5; 0xd6;
+                           (* VPMULLW (%_% ymm10) (%_% ymm4) (%_% ymm14) *)
+  0xc5; 0xfd; 0xe5; 0xff;  (* VPMULHW (%_% ymm7) (%_% ymm0) (%_% ymm7) *)
+  0xc4; 0x41; 0x7d; 0xe5; 0xc9;
+                           (* VPMULHW (%_% ymm9) (%_% ymm0) (%_% ymm9) *)
+  0xc4; 0x41; 0x7d; 0xe5; 0xc0;
+                           (* VPMULHW (%_% ymm8) (%_% ymm0) (%_% ymm8) *)
+  0xc4; 0x41; 0x7d; 0xe5; 0xd2;
+                           (* VPMULHW (%_% ymm10) (%_% ymm0) (%_% ymm10) *)
+  0xc5; 0x5d; 0xe5; 0xda;  (* VPMULHW (%_% ymm11) (%_% ymm4) (%_% ymm2) *)
+  0xc5; 0x55; 0xe5; 0xe2;  (* VPMULHW (%_% ymm12) (%_% ymm5) (%_% ymm2) *)
+  0xc5; 0x4d; 0xe5; 0xeb;  (* VPMULHW (%_% ymm13) (%_% ymm6) (%_% ymm3) *)
+  0xc5; 0x5d; 0xe5; 0xf3;  (* VPMULHW (%_% ymm14) (%_% ymm4) (%_% ymm3) *)
+  0xc5; 0xa5; 0xf9; 0xff;  (* VPSUBW (%_% ymm7) (%_% ymm11) (%_% ymm7) *)
+  0xc4; 0x41; 0x1d; 0xf9; 0xc9;
+                           (* VPSUBW (%_% ymm9) (%_% ymm12) (%_% ymm9) *)
+  0xc4; 0x41; 0x3d; 0xf9; 0xc5;
+                           (* VPSUBW (%_% ymm8) (%_% ymm8) (%_% ymm13) *)
+  0xc4; 0x41; 0x0d; 0xf9; 0xd2;
+                           (* VPSUBW (%_% ymm10) (%_% ymm14) (%_% ymm10) *)
+  0xc5; 0xbd; 0xfd; 0xff;  (* VPADDW (%_% ymm7) (%_% ymm8) (%_% ymm7) *)
+  0xc4; 0x41; 0x2d; 0xfd; 0xc9;
+                           (* VPADDW (%_% ymm9) (%_% ymm10) (%_% ymm9) *)
+  0xc5; 0xfd; 0x7f; 0xbf; 0xc0; 0x01; 0x00; 0x00;
+                           (* VMOVDQA (Memop Word256 (%% (rdi,448))) (%_% ymm7) *)
+  0xc5; 0x7d; 0x7f; 0x8f; 0xe0; 0x01; 0x00; 0x00;
+                           (* VMOVDQA (Memop Word256 (%% (rdi,480))) (%_% ymm9) *)
   0xc3                     (* RET *)
 ];;
 
-let mlkem_basemul_k2_tmc = define_trimmed "mlkem_basemul_k2_tmc" mlkem_basemul_k2_mc;;
-let mlkem_basemul_k2_tmc_EXEC = X86_MK_CORE_EXEC_RULE mlkem_basemul_k2_tmc;;
+let mlkem_basemul_k2_tmc2 = define_trimmed "mlkem_basemul_k2_tmc2" mlkem_basemul_k2_mc2;;
+let mlkem_basemul_k2_tmc2_EXEC = X86_MK_CORE_EXEC_RULE mlkem_basemul_k2_tmc2;;
 
 (* Enable simplification of word_subwords by default.
    Nedded to prevent the symbolic simulation to explode
@@ -164,37 +434,39 @@ let SIMPLE_SPEC = prove(
         aligned 32 src2t /\
         aligned 32 dst /\
         ALL (nonoverlapping (dst, 512))
-            [(word pc, 276);
+            [(word pc, 1152);
              (src1, 1024); (src2, 1024); (src2t, 512)]
         ==> ensures x86
-              (\s. bytes_loaded s (word pc) (BUTLAST mlkem_basemul_k2_tmc) /\
+              (\s. bytes_loaded s (word pc) (BUTLAST mlkem_basemul_k2_tmc2) /\
                    read RIP s = word pc /\
                    C_ARGUMENTS [dst; src1; src2; src2t] s /\
-                   (!i. i < 16 ==> !j. j < 2
+                   (!i. i < 16 ==> !j. j < 8
                         ==> read(memory :> bytes16
                              (word_add src1 (word (64*j + 2*i)))) s = a i j) /\
-                   (!i. i < 16 ==> !j. j < 2
+                   (!i. i < 16 ==> !j. j < 8
                         ==> read(memory :> bytes16
                              (word_add src1 (word (64*j + 32 + 2*i)))) s = b i j) /\
-                   (!i. i < 16 ==> !j. j < 2
+                   (!i. i < 16 ==> !j. j < 8
                         ==> read(memory :> bytes16
                              (word_add src2 (word (64*j + 2*i)))) s = c i j) /\
-                   (!i. i < 16 ==> !j. j < 2
+                   (!i. i < 16 ==> !j. j < 8
                         ==> read(memory :> bytes16
                              (word_add src2 (word (64*j + 32 + 2*i)))) s = d i j) /\
-                   (!i. i < 16 ==> !j. j < 2
+                   (!i. i < 16 ==> !j. j < 8
                         ==> read(memory :> bytes16
                              (word_add src2t (word (32*j + 2*i)))) s = dz i j))
-              (\s. read RIP s = word (pc + 276) /\
-                   (!i. i < 16
-                        ==> read(memory :> bytes16
-                             (word_add dst (word (2*i)))) s =
-                                montmuladd_x86 (b i 0) (dz i 0) (a i 0) (c i 0)) /\
-                   (!i. i < 16
-                        ==> read(memory :> bytes16
-                             (word_add dst (word (64 + 2*i)))) s =
-                                montmuladd_odd_x86 (b i 1) (dz i 1) (a i 1) (c i 1)) /\
-                   (!i. i < 16 ==> !j. j < 2
+              (\s. read RIP s = word (pc + 1152) /\
+                   (!i. i < 16 ==> !j. j < 4
+                        ==> (let j' = 2*j in
+                        read(memory :> bytes16
+                             (word_add dst (word (64*j' + 2*i)))) s =
+                                montmuladd_x86 (b i j') (dz i j') (a i j') (c i j'))) /\
+                   (!i. i < 16 ==> !j. j < 4
+                        ==> (let j' = 2*j+1 in
+                        read(memory :> bytes16
+                             (word_add dst (word (64*j' + 2*i)))) s =
+                                montmuladd_odd_x86 (b i j') (dz i j') (a i j') (c i j'))) /\
+                   (!i. i < 16 ==> !j. j < 8
                         ==> read(memory :> bytes16
                              (word_add dst (word (64*j + 32 + 2*i)))) s =
                                 montmuladd_x86 (b i j) (c i j) (a i j) (d i j)))
@@ -203,7 +475,7 @@ let SIMPLE_SPEC = prove(
                MAYCHANGE [memory :> bytes(dst, 512)])`,
 
   REWRITE_TAC [MAYCHANGE_REGS_AND_FLAGS_PERMITTED_BY_ABI;
-    NONOVERLAPPING_CLAUSES; ALL; C_ARGUMENTS; fst mlkem_basemul_k2_tmc_EXEC] THEN
+    NONOVERLAPPING_CLAUSES; ALL; C_ARGUMENTS; fst mlkem_basemul_k2_tmc2_EXEC] THEN
   REPEAT STRIP_TAC THEN
 
   GHOST_INTRO_TAC `init_ymm0:int256` `read YMM0` THEN
@@ -226,10 +498,10 @@ let SIMPLE_SPEC = prove(
   (* Symbolically run one instruction *)
   (let lemma = WORD_BLAST
   `(word_zx:int256->int128) x = word_subword x (0,128)` in
-  MAP_EVERY (fun n -> X86_STEPS_TAC mlkem_basemul_k2_tmc_EXEC [n] THEN
+  MAP_EVERY (fun n -> X86_STEPS_TAC mlkem_basemul_k2_tmc2_EXEC [n] THEN
                       RULE_ASSUM_TAC(REWRITE_RULE[lemma]) THEN
                       SIMD_SIMPLIFY_TAC [montmul_x86; montmuladd_x86; montmul_odd_x86; montmuladd_odd_x86])
-            (1--60)) THEN
+            (1--222)) THEN
 
   ENSURES_FINAL_STATE_TAC THEN
   ASM_REWRITE_TAC[] THEN
@@ -240,7 +512,11 @@ let SIMPLE_SPEC = prove(
   check (can (term_match [] `read qqq s:int256 = xxx`) o concl))) THEN
 
   CONV_TAC(TOP_DEPTH_CONV EXPAND_CASES_CONV) THEN
-  CONV_TAC(TOP_DEPTH_CONV NUM_MULT_CONV THENC
-           TOP_DEPTH_CONV NUM_ADD_CONV) THEN
+  CONV_TAC(DEPTH_CONV NUM_MULT_CONV THENC
+           DEPTH_CONV NUM_ADD_CONV THENC
+           DEPTH_CONV let_CONV) THEN
+  CONV_TAC(DEPTH_CONV NUM_MULT_CONV THENC
+           DEPTH_CONV NUM_ADD_CONV THENC
+           DEPTH_CONV let_CONV) THEN
   ASM_REWRITE_TAC[WORD_ADD_0]
 );;
